aneris/examples/transactional_consistency/wrapped_library.v
@@ -1,39 +1,55 @@
 From aneris.aneris_lang Require Import ast.
 From aneris.examples.transactional_consistency Require Import code_api.
 
-Definition start_emit_event : val := 
-  λ: "cst", ("cst", #"St").
+Definition start_pre_emit_event : val := 
+  λ: "cst", ("cst", #"StPre").
+
+Definition start_post_emit_event : val := 
+  λ: "cst", ("cst", #"StPost").
 
 Definition wrap_start (start : val) : val := 
   λ: "cst", 
+  let: "tag" := Fresh (start_pre_emit_event "cst") in 
   start "cst" ;;
-  Fresh (start_emit_event "cst") ;;
+  Emit ("tag" , start_post_emit_event "cst") ;;
   #().
 
-Definition read_emit_event : val :=
-  λ: "cst" "key" "vo", ("cst", (#"Rd", ("key", "vo"))).
+Definition read_pre_emit_event : val := 
+  λ: "cst", ("cst", #"RdPre").
+
+Definition read_post_emit_event : val :=
+  λ: "cst" "key" "vo", ("cst", (#"RdPre", ("key", "vo"))).
 
 Definition wrap_read (read : val) : val := 
   λ: "cst" "k", 
+  let: "tag" := Fresh (read_pre_emit_event "cst") in
   let: "vo" := read "cst" "k" in 
-  Fresh (read_emit_event "cst" "k" "vo") ;;
+  Emit ("tag" ,read_post_emit_event "cst" "k" "vo") ;;
   "vo".
 
-Definition write_emit_event : val :=
-  λ: "cst" "key" "v", ("cst", (#"Wr", ("key", "v"))).
+Definition write_pre_emit_event : val := 
+  λ: "cst", ("cst", #"WrPre").
+
+Definition write_post_emit_event : val :=
+  λ: "cst" "key" "v", ("cst", (#"WrPost", ("key", "v"))).
 
 Definition wrap_write (write : val) : val := 
   λ: "cst" "k" "v", 
-  Fresh (write_emit_event "cst" "k" "v") ;;
-  write "cst" "k" "v".
+  let: "tag" := Fresh (write_pre_emit_event "cst") in 
+  write "cst" "k" "v" ;;
+  Emit ("tag", write_post_emit_event "cst" "k" "v").
 
-Definition commit_emit_event : val :=
-  λ: "cst" "b", ("cst", (#"Cm", "b")).
+Definition commit_pre_emit_event : val := 
+  λ: "cst", ("cst", #"CmPre").
+
+Definition commit_post_emit_event : val :=
+  λ: "cst" "b", ("cst", (#"CmPost", "b")).
 
 Definition wrap_commit (commit : val) : val := 
   λ: "cst", 
+  let: "tag" := Fresh (commit_pre_emit_event "cst") in 
   let: "b" := commit "cst" in 
-  Fresh (commit_emit_event "cst" "b") ;; 
+  Emit ("tag", commit_post_emit_event "cst" "b") ;; 
   "b".
   
 Global Instance KVS_wrapped_api (lib : KVS_transaction_api) :
